common/UCComposition.ec
@@ -1,0 +1,116 @@
+(* Composition Theorem Definitions and Proofs *)
+
+require import UCCore UCListAux.
+
+abstract theory CompRF.
+
+(* begin theory parameters *)
+
+op rf_info : rf_info.
+
+axiom rf_info_valid : rf_info_valid rf_info.
+
+op change_pari : int.  (* parameter being changed from real to ideal *)
+
+axiom change_pari_valid : 1 <= change_pari <= rf_info.`rfi_num_params.
+
+(* end theory parameters *)
+
+module MakeRFComp (Rest : FUNC, Par : FUNC) : FUNC = {
+  var self : addr
+
+  proc init(_self : addr) : unit = {
+    self <- _self;
+    Rest.init(_self);
+    Par.init(_self ++ [change_pari]);
+  }
+
+  proc after_core_or_par(r : msg option, orig_dest_addr)
+         : msg option * msg * bool = {
+    var m : msg <- witness; var pari : int;
+    var not_done <- true;
+    if (r = None) {
+      not_done <- false;
+    }
+    else {
+      m <- oget r;  (* next iteration, if any, will use m *)
+      if (m.`3.`1 <> orig_dest_addr) {
+        not_done <- false; r <- None;
+      }
+      elif (m.`1 = Dir) {
+        if (m.`3.`1 = self) {
+          if (envport self m.`2) {
+            not_done <- false;
+          }
+          elif (! (addr_eq_param rf_info self m.`2.`1 \/
+                   addr_eq_subfun rf_info self m.`2.`1)) {
+            not_done <- false; r <- None;
+          }
+        }
+        elif (addr_eq_param rf_info self m.`3.`1 \/
+              addr_eq_subfun rf_info self m.`3.`1) {
+          if (m.`2.`1 <> self) {
+            not_done <- false; r <- None;
+          }
+        }
+        else {  (* should not happen *)
+          not_done <- false; r <- None;
+        }
+      }
+      else {  (* m.`1 = Adv *)
+        not_done <- false;
+        if (m.`2.`1 <> adv) {
+          r <- None;
+        }
+        elif (m.`3.`1 = self \/
+              addr_eq_subfun rf_info self m.`3.`1) {
+          if (! rf_info.`rfi_adv_pi_begin + 1 <= m.`2.`2 <=
+                rf_info.`rfi_adv_pi_main_end) {
+            r <- None;
+          }
+        }
+        elif (addr_ge_param rf_info self m.`3.`1) {
+          pari <- head_of_drop_size_first 0 self m.`3.`1;
+          if (! (nth 0 rf_info.`rfi_adv_pi_begin_params pari < m.`2.`2 <=
+                 nth 0 rf_info.`rfi_adv_pi_end_params pari)) {
+            r <- None;
+          }
+        }
+        else {  (* should not happen *)
+          r <- None;
+        }
+      }
+    }          
+    return (r, m, not_done);
+  }
+
+  proc loop(m : msg) : msg option = {
+    var r : msg option <- None;
+    var not_done : bool <- true;
+    while (not_done) {
+      if (self ++ [change_pari] <= m.`2.`1) {
+        r <@ Par.invoke(m);
+      }
+      else {
+        r <@ Rest.invoke(m);
+      }
+      (r, m, not_done) <@ after_core_or_par(r, m.`2.`1);
+    }
+    return r;
+  }
+
+  proc invoke(m : msg) : msg option = {
+    var r : msg option <- None;
+    (* we can assume m.`3.`1 is not >= self *)
+    if ((m.`1 = Dir /\ m.`2.`1 = self) \/
+        (m.`1 = Adv /\
+         (m.`2.`1 = self \/
+          addr_ge_param rf_info self m.`2.`1 \/
+          addr_eq_subfun rf_info self m.`2.`1))) {
+      r <@ loop(m);
+    }
+    return r;
+  }
+}.
+
+end CompRF.
